BB_sem_while_equiv.v
@@ -18,6 +18,7 @@ Require Import Coq.Lists.List.
 Require Import Main.BB_denotations.
 Require Import Main.BB_aux_proof.
 Require Import Main.BB_gen_properties.
+Require Import Main.utils.
 
 Import Denotation.
 Import EDenote.
